hol/bdd_gen_mergeScript.sml
@@ -51,6 +51,8 @@ QED
 
 
         
+
+        
 Theorem merge_lookup_exists:
   ∀ edges n n' n'' x.        
     n' ≠ n'' ∧
@@ -70,8 +72,6 @@ Proof
 QED
 
 
-        
-        
 Theorem mergable_correct_leaf:
   ∀labels n'' r edges n' n mv b rec.
     BDD_WF (r,edges,labels) ∧
@@ -165,13 +165,13 @@ QED
 
 Theorem merge_edges_res:        
   ∀ edges n n' n'' nr nl r labels.
-    mergable  (r,edges,labels) n n' ∧
+    (mergable (r,edges,labels) n n' ∨ eleminatble (r,edges,labels) n n') ∧
     n'' ≠ n' ∧
     ALOOKUP (merge_edges edges n n') n'' = SOME (nr,nl) ⇒
     (nr ≠ n' ∧ nl ≠ n')
 Proof   
   rpt strip_tac >>
-  gvs[mergable_def] >>
+  gvs[mergable_def, eleminatble_def] >>
   metis_tac[merge_edges_glue]
 QED        
 
@@ -348,34 +348,6 @@ Proof
   fs[AllCaseEqs()]
 QED
 
-        
-(*
-Theorem merge_replaces_stays_same:            
-∀ edges n' n x1 x2 x1' x2'.
-n' ≠ x1' ∧ n' ≠ x2' ∧
-ALOOKUP (merge_edges edges n n') n = SOME (x1,x2) ∧
-ALOOKUP edges n = SOME (x1',x2') ⇒
-(x1=x1' ∧ x2=x2')
-Proof
-         
-Induct >-
- gvs[merge_edges_def] >>
-rpt strip_tac >>
-(
-gvs[Once merge_edges_list_cons] >>
-fs[ALOOKUP_APPEND] >>
-Cases_on ‘ALOOKUP (merge_edges [h] n n') n’ >> gvs[] >|[
-    PairCases_on ‘h’ >>
-    imp_res_tac merge_Theorem1 >>
-    rgs[Once ALOOKUP_def] >>
-    metis_tac[]
-    ,
-    metis_tac[merge_replaces_stays_same_singular]
-  ]
-)
-                                                       
-QED
-*)
 
 
 (* very slow proof, check why*)       
@@ -410,11 +382,12 @@ QED
 
     
 
-                                                
+(* fails *)                                                
 Theorem mergable_correct_internal:
-  ∀ x vars_consumed  r edges labels n n' n'' nl nr pred mv b rec.
+  ∀ x vars_consumed  vars r edges labels n n' n'' nl nr pred mv b rec.
     consumed_dom_bdd vars_consumed (r,edges,labels) ∧
-    mv_dom_bdd mv (r,edges,labels) ∧
+    fv_in_BDD rec (r,edges,labels) (vars ⧺ vars_consumed)∧
+    mv_dom_vars mv (vars ⧺ vars_consumed) ∧
     BDD_ordered (r,edges,labels) vars_consumed ∧
     BDD_WF (r,edges,labels) ∧
     mergable (r,edges,labels) n n' ∧
@@ -425,6 +398,7 @@ Theorem mergable_correct_internal:
     (BDD_sem rec (r,edges,labels) mv n'' b ⇔
        BDD_sem rec (r,ADELKEY n' (merge_edges edges n n'),ADELKEY n' labels) mv n'' b)
 Proof
+        
   ntac 2 strip_tac >>
   measureInduct_on `THE(INDEX_OF x vars_consumed)` >>
   rpt strip_tac >>
@@ -469,7 +443,7 @@ Proof
             
             first_x_assum (strip_assume_tac o (Q.SPECL [‘INDEX_OF (x':string) (vars_consumed: string list)’])) >>
             rgs[PULL_FORALL] >>  
-            first_x_assum (strip_assume_tac o (Q.SPECL [‘x'’, ‘vars_consumed’, ‘r’, ‘edges’, ‘labels’, ‘n’, ‘n'’,
+            first_x_assum (strip_assume_tac o (Q.SPECL [‘x'’, ‘vars_consumed’, ‘vars’, ‘r’, ‘edges’, ‘labels’, ‘n’, ‘n'’,
                                                         ‘nr’, ‘r'’, ‘q’,  ‘pred'’, ‘mv’, ‘b’])) >>
             gvs[] >>
             
@@ -518,7 +492,7 @@ Proof
                       rename1 ‘SOME (nl_old,nr_old) = ALOOKUP edges n'’ >>
                       rename1 ‘ALOOKUP (merge_edges edges n n') n = SOME (n1,n2)’ >>
                       subgoal ‘∃ bool . ALOOKUP mv x' = SOME bool’>-
-                              (gvs[mv_dom_bdd_def, lookup_is_some_def] >> res_tac >> gvs[]) >>
+                       (  imp_res_tac consumed_dom_bdd_in_mv >> gvs[] ) >>
                               
                           Cases_on ‘bool’ >> (
                               
@@ -543,7 +517,7 @@ Proof
                              
                               first_x_assum (strip_assume_tac o (Q.SPECL [‘INDEX_OF (x':string) (vars_consumed: string list)’])) >>
                               gvs[PULL_FORALL] >>
-                              first_x_assum (strip_assume_tac o (Q.SPECL [‘x'’, ‘vars_consumed’, ‘r’, ‘edges’, ‘labels’, ‘n’,
+                              first_x_assum (strip_assume_tac o (Q.SPECL [‘x'’, ‘vars_consumed’, ‘vars’, ‘r’, ‘edges’, ‘labels’, ‘n’,
                                                                           ‘n'’, ‘n’, ‘nr_old’, ‘n1’,  ‘r'’, ‘mv’, ‘b’])) >>
                               rgs[] >>
                               
@@ -578,7 +552,7 @@ Proof
             
             first_x_assum (strip_assume_tac o (Q.SPECL [‘INDEX_OF (x':string) (vars_consumed: string list)’])) >>
             rgs[PULL_FORALL] >>  
-            first_x_assum (strip_assume_tac o (Q.SPECL [‘x'’, ‘vars_consumed’, ‘r’, ‘edges’, ‘labels’, ‘n’, ‘n'’,
+            first_x_assum (strip_assume_tac o (Q.SPECL [‘x'’, ‘vars_consumed’, ‘vars’, ‘r’, ‘edges’, ‘labels’, ‘n’, ‘n'’,
                                                         ‘nl’, ‘r'’, ‘q’,  ‘pred'’, ‘mv’, ‘b’])) >>
             gvs[] >>
             
@@ -624,7 +598,7 @@ Proof
                       rename1 ‘SOME (nl_old,nr_old) = ALOOKUP edges n'’ >>
                       rename1 ‘ALOOKUP (merge_edges edges n n') n = SOME (n1,n2)’ >>
                       subgoal ‘∃ bool . ALOOKUP mv x' = SOME bool’>-
-                              (gvs[mv_dom_bdd_def, lookup_is_some_def] >> res_tac >> gvs[]) >>
+                              (imp_res_tac consumed_dom_bdd_in_mv >> gvs[]) >>
                               
                           Cases_on ‘bool’ >> (
                               
@@ -649,7 +623,7 @@ Proof
                              
                               first_x_assum (strip_assume_tac o (Q.SPECL [‘INDEX_OF (x':string) (vars_consumed: string list)’])) >>
                               gvs[PULL_FORALL] >>
-                              first_x_assum (strip_assume_tac o (Q.SPECL [‘x'’, ‘vars_consumed’, ‘r’, ‘edges’, ‘labels’, ‘n’,
+                              first_x_assum (strip_assume_tac o (Q.SPECL [‘x'’, ‘vars_consumed’, ‘vars’, ‘r’, ‘edges’, ‘labels’, ‘n’,
                                                                           ‘n'’, ‘n’, ‘nr_old’, ‘n1’,  ‘r'’, ‘mv’, ‘b’])) >>
                               rgs[] >>
                               
@@ -674,11 +648,12 @@ QED
 
 
              
-             
+           
 Theorem Lemma3:
-  ∀ labels vars_consumed n'' r edges n' n mv b rec.
+  ∀ labels vars vars_consumed n'' r edges n' n mv b rec.
     consumed_dom_bdd vars_consumed (r,edges,labels) ∧
-    mv_dom_bdd mv (r,edges,labels) ∧
+    fv_in_BDD rec (r,edges,labels) (vars++vars_consumed) ∧
+    mv_dom_vars mv (vars ⧺ vars_consumed) ∧
     BDD_ordered (r,edges,labels) vars_consumed ∧
     BDD_WF (r,edges,labels) ∧
     mergable (r,edges,labels) n n' ∧
@@ -710,33 +685,13 @@ Proof
 QED
 
 
-
-Theorem mv_dom_bdd_merge_preserved:
-  ∀ r edges labels keys n n' mv.   
-    mergable (r,edges,labels) n n' ∧
-    mv_dom_bdd mv (r,ADELKEY n' (merge_edges edges n n'),ADELKEY n' labels) ⇒
-    mv_dom_bdd mv (r,edges,labels)
-Proof
-  rpt strip_tac >>
-  gvs[mv_dom_bdd_def] >>
-  rpt strip_tac >>
-  Cases_on ‘n'' = n'’ >|[
-    rgs[mergable_def] >>
-    gvs[ALOOKUP_ADELKEY] >>
-    res_tac >> gvs[]
-    ,
-    gvs[ALOOKUP_ADELKEY] >>
-    res_tac >> gvs[]            
-  ]
-QED
-
-
+        
 
 Theorem fv_in_labels_preserved:        
-  ∀ r edges labels keys n n' mv rec. 
+  ∀ r edges labels keys n n' varslist rec. 
     mergable (r,edges,labels) n n' ∧        
-    fv_in_labels rec (ADELKEY n' labels) mv  ⇒         
-    fv_in_labels rec labels mv
+    fv_in_labels rec (ADELKEY n' labels) varslist  ⇒         
+    fv_in_labels rec labels varslist
 Proof
   rpt strip_tac >>
   gvs[fv_in_labels_def] >>
@@ -767,17 +722,19 @@ QED
 
 
 
-                           
+
+
         
 Theorem merge_correct:        
-  ∀ r edges labels vars_consumed n n' rec .
-    correct_sem rec (r,edges,labels) ∧
+  ∀ r edges labels vars vars_consumed n n' rec.
+    correct_sem rec (r,edges,labels) (vars++vars_consumed)  ∧
     BDD_WF (r,edges,labels) ∧
     consumed_dom_bdd vars_consumed (r,edges,labels) ∧
-    BDD_ordered (r,edges,labels) vars_consumed ∧           
+    BDD_ordered (r,edges,labels) vars_consumed ∧
+    fv_in_BDD rec (r,edges,labels) (vars++vars_consumed)  ∧
     mergable (r,edges,labels) n n'
     ==>
-    correct_sem rec (merge (r,edges,labels) n n')
+    correct_sem rec (merge (r,edges,labels) n n') (vars++vars_consumed)
 Proof
   rpt strip_tac >>   
   simp[Once correct_sem_def] >>
@@ -795,15 +752,10 @@ Proof
     ,
     
     assume_tac Lemma3 >>
-    first_x_assum (strip_assume_tac o (Q.SPECL [‘labels’, ‘vars_consumed’, ‘n''’, ‘r’, ‘edges’, ‘n'’, ‘n’, ‘mv’, ‘b’, ‘rec’])) >>
+    first_x_assum (strip_assume_tac o (Q.SPECL [‘labels’, ‘vars’, ‘vars_consumed’, ‘n''’, ‘r’, ‘edges’, ‘n'’, ‘n’, ‘mv’, ‘b’, ‘rec’])) >>
     gvs[] >>
 
-    
-    ‘mv_dom_bdd mv (r,edges,labels)’ by metis_tac[mv_dom_bdd_merge_preserved] >>
-    res_tac >>
 
-    ‘fv_in_labels rec labels mv’ by metis_tac [fv_in_labels_preserved] >>
-                
     gvs[correct_sem_def] >>
     res_tac >>
     
@@ -827,76 +779,682 @@ QED
 (*                  E L I M I N A T E                  *)
 (*                                                     *)
 (*******************************************************)
-
-(* move to genScript *)        
-Definition eleminatble_def:        
-eleminatble ((r,edges,labels):('a,'b)BDD)  n n' = 
-(n≠n' ∧ ALOOKUP edges n' = SOME (n,n) )
-End
-
-
-(*******************************************************)
-(*    Definition of eliminate is the same as  merge    *)
-(*******************************************************)
-
-(*         
-Definition eliminate_edges_def:
-  eliminate_edges (edges:edges) n n' =
-   MAP (\(a,b,c). ( a, if (b=n' ∧ c=n') then (n,n)
-                 else if (b=n') then (n,c)
-                 else if (c=n') then (b,n)
-                     else (b,c))) edges 
-End
-
-
-
-Definition eliminate_def:
-  eliminate ((r,edges,labels):BDD) n n' =
-  let edges' = merge_edges (edges:edges) n n' in
-    let edges'' = ADELKEY n' edges' in
-      let labels' = ADELKEY n' labels in
-          (r,edges'',labels')
-End
-
-
-
-       
-EVAL “eleminatble (1,[(0,1,5);(1,2,2);(2,3,4)],[]) 2 1”
-EVAL “eliminate_edges [(0,1,5);(1,2,2);(2,3,4)] 2 1”
-EVAL “eliminate (1,[(0,1,5);(1,2,2);(2,3,4)],[]) 2 1”
-
-
-mergable_def     
-EVAL “mergable (0,[(0,1,5);(1,2,2);(5,2,2)],[(1,x);(5,x)]) 1 5”
-EVAL “merge_edges [(0,1,5);(1,2,2);(5,2,2)] 1 5”
-
-EVAL “eleminatble (0,[(0,1,5);(1,2,2);(5,2,2)],[(1,x);(5,x)]) 2 1”
-EVAL “eliminate_edges [(0,1,5);(1,2,2);(5,2,2)] 2 1”
-EVAL “eliminate (0,[(0,1,5);(1,2,2);(5,2,2)],[(1,x);(5,x)]) 2 1”
-
-
-EVAL “eleminatble (0,[(1,2,2)],[(1,x);(5,x)]) 2 1”
-EVAL “eliminate_edges [(1,2,2)] 2 1”
-EVAL “eliminate (0,[(1,2,2)],[(1,x);(5,x)]) 2 1”
-
-
-EVAL “eleminatble (0,[(1,2,2);(2,3,4)],[(1,x);(5,x)]) 2 1”
-EVAL “eliminate_edges [(1,2,2);(2,3,4)] 2 1”
-EVAL “eliminate (0,[(1,2,2);(2,3,4)],[(1,x);(5,x)]) 2 1”
-
-
-
-EVAL “eleminatble (0,[(1,2,2)],[(1,x);(5,x)]) 2 1”
-EVAL “eliminate_edges [(1,2,2)] 2 1”
-EVAL “eliminate (0,[(1,2,2)],[(1,x);(5,x)]) 2 1”
-
      
+
+
+
+Definition is_unique_var_def:
+  is_unique_var labels n =
+    case ALOOKUP labels n of
+      | SOME (non_termn (SOME x, _)) =>
+          EVERY (λ(n', lbl).
+              (case lbl of
+               | non_termn (SOME x', _) => (x' ≠ x)
+               | _ => T
+              )
+                ) (ADELKEY n labels)
+      | _ => T
+End
+
+
+
+
+Theorem not_unique_exsists_labels:        
+  ∀ labels n x p.
+    ALL_DISTINCT (MAP FST labels) ∧ 
+    ALOOKUP labels n = SOME (non_termn (SOME x,p)) ∧
+    ¬is_unique_var labels n ⇒
+    ∃ n' p'. n' ≠ n ∧ ALOOKUP labels n' = SOME (non_termn (SOME x,p'))
+Proof      
+  Induct >>
+  rpt strip_tac >>
+  gvs[] >>
+  PairCases_on ‘h’ >> gvs[] >>
+  gvs[AllCaseEqs()] >|[
+    
+    rgs[Once is_unique_var_def, Once EXISTS_MEM] >>
+    PairCases_on ‘e’ >> gvs[] >>
+    rpt (BasicProvers.FULL_CASE_TAC >> rgs[]) >>
+    qexistsl_tac [‘e0’, ‘r’] >>
+    gvs[] >>
+    imp_res_tac ALOOKUP_ALL_DISTINCT_MEM    
+    ,
+
+    rgs[is_unique_var_def] >>
+    rgs[Once EXISTS_MEM] >>
+    
+    PairCases_on ‘e’ >> gvs[] >>
+    rpt (BasicProvers.FULL_CASE_TAC >> rgs[]) >|[
+        
+        qexistsl_tac [‘e0’, ‘r’] >> gvs[] >>
+        imp_res_tac ALOOKUP_ALL_DISTINCT_MEM >>
+        gvs[]
+        ,
+        
+        gvs[] >>        
+        res_tac >>
+        rpt (BasicProvers.FULL_CASE_TAC >> rgs[]) >>
+        imp_res_tac ALOOKUP_ALL_DISTINCT_MEM >>
+        qexistsl_tac [‘e0’, ‘r’] >> gvs[] >>
+        Cases_on ‘h0 = e0’ >> gvs[] >>
+        imp_res_tac mem_fst_snd >> gvs[]
+      ]
+  ]
+QED        
+
+
+
+
+Theorem leaf_lbl_is_unique:
+  ∀ labels n action p p'.
+    (ALOOKUP labels n = SOME (non_termn (NONE,p)) ∨ ALOOKUP labels n = SOME (termn (action,p'))) ⇒
+    is_unique_var labels n
+Proof
+  rpt strip_tac >>
+  rgs[Once is_unique_var_def]
+QED
+
+
+
+
+
+                     
+(*       
+Theorem mv_dom_bdd_eliminate_preserved:
+  ∀ r edges labels keys n n' mv.
+    ALL_DISTINCT (MAP FST labels) ∧
+    eleminatble (r,edges,labels) n n' ∧
+    ~is_unique_var labels n' ∧
+    mv_dom_bdd mv (merge (r,edges,labels) n n') ⇒
+    mv_dom_bdd mv (r,edges,labels)
+Proof
+
+  rpt strip_tac >>
+  gvs[merge_def] >>
+  gvs[mv_dom_bdd_def] >>
+  rpt strip_tac >>
+  Cases_on ‘n'' = n'’ >> gvs[] >|[
+    rgs[eleminatble_def] >>
+    gvs[ALOOKUP_ADELKEY] >>
+    imp_res_tac not_unique_exsists_labels >>
+    res_tac >> gvs[]
+    ,
+    gvs[ALOOKUP_ADELKEY] >>
+    res_tac >> gvs[]            
+  ]
+QED
+
 *)
+
+        
+Theorem sem_imp_label_lookup_some:        
+  ∀ r edges labels n mv b rec.
+    BDD_sem rec (r,edges,labels) mv n b ⇒
+    lookup_is_some labels n
+Proof      
+  Induct_on ‘BDD_sem’ >>
+  rpt strip_tac >>
+  rgs[Once BDD_sem_cases, lookup_is_some_def]
+QED
+
+
+
+
+
+
+
+        
+
+Theorem look_some_in_delkey_imp_og:
+  ∀ labels n n'.
+    n ≠ n' ⇒
+    (lookup_is_some (ADELKEY n labels) n' ⇔
+       lookup_is_some labels n')
+Proof
+  Induct >>
+  rpt strip_tac >>
+  gvs[lookup_is_some_def, ALOOKUP_ADELKEY]
+QED
+
+
+Theorem alookup_delkey_imp_og:
+  ∀ l n n' x.
+    n ≠ n' ⇒
+    (ALOOKUP (ADELKEY n l) n' = SOME x ) ⇒
+    (ALOOKUP l n' = SOME x)
+Proof
+  Induct >>
+  rpt strip_tac >>
+  gvs[lookup_is_some_def, ALOOKUP_ADELKEY]
+QED
+
+
+Theorem delkey_alookup_imp_og:
+  ∀ l n n' x.
+    n ≠ n' ⇒
+    (ALOOKUP l n' = SOME x) ⇒
+             (ALOOKUP (ADELKEY n l) n' = SOME x )
+Proof
+Induct >>
+rpt strip_tac >>
+gvs[lookup_is_some_def, ALOOKUP_ADELKEY]
+QED
+        
+
+Theorem op_sem_adel_key:
+  ∀ labels n' n'' mv rec.
+    n' ≠ n'' ⇒        
+    (op_sem rec (get_prop (ADELKEY n' labels) n'') mv = op_sem rec (get_prop labels n'') mv)
+Proof                                  
+  rpt strip_tac >>
+  gvs[op_sem_def, get_prop_def] >>
+  gvs[AllCaseEqs()]>>
+  Cases_on ‘ALOOKUP (ADELKEY n' labels) n''’ >> gvs[ALOOKUP_ADELKEY] >>
+  Cases_on ‘x’ >> gvs[ALOOKUP_ADELKEY] >>
+  Cases_on ‘p’ >> gvs[]
+QED
+
+
+
+
+Theorem eliminatable_is_internal_indeed:        
+  ∀ r edges labels n n'.
+    BDD_WF (r,edges,labels) ∧        
+    eleminatble (r,edges,labels) n n' ⇒
+    ∃ x p . ALOOKUP labels n'= SOME (non_termn(SOME x,p)) 
+Proof
+  rpt strip_tac >>
+  rgs[eleminatble_def] >>
+  ‘MEM n' (dom_range_edges edges)’ by metis_tac[lookup_edges_in_domain] >> 
+  rgs[BDD_WF_def, lookup_is_some_def, is_lookup_internal_def] >>
+  res_tac >> gvs[] 
+QED
+
+
+
+(*
+Theorem mv_dom_bdd_del_element_added:
+  ∀ r labels edges mv n n' x p b'.  
+    ALOOKUP labels n' = SOME (non_termn (SOME x,p)) ∧        
+    mv_dom_bdd mv (r,ADELKEY n' (merge_edges edges n n'),ADELKEY n' labels) ⇒
+    mv_dom_bdd (mv ⧺ [(x,b')]) (r,edges,labels)
+Proof
+  rpt strip_tac >>
+  gvs[mv_dom_bdd_def] >>
+  rpt strip_tac >>
+  Cases_on ‘n'' = n'’ >>
+  rgs[mergable_def] >>
+  gvs[ALOOKUP_ADELKEY] >>
+  res_tac >> gvs[] >>
+  
+  Cases_on ‘n=n'’ >>
+  gvs[lookup_is_some_def] >>
+  
+  gvs[ALOOKUP_APPEND] >>
+  gvs[AllCaseEqs()]>>
+  Cases_on ‘ALOOKUP mv x’ >> gvs[]              
+QED
+*)
+
+
+Theorem fv_mv_extended_x:
+  ∀ p mv x b rec.        
+    fv_in_p rec p mv ⇒
+    fv_in_p rec p (mv ⧺ [(x,b)])
+Proof
+  rpt strip_tac >>
+  rgs[fv_in_p_def] >>
+  rpt strip_tac >>
+  res_tac >>
+  gvs[ALOOKUP_APPEND]
+QED
+     
+
+
+
+Theorem merge_edges_elim_same_helper_l:
+  ∀ h n n' n1 n2 n1' n2'.
+    n1 ≠ n ∧    
+    ALOOKUP (merge_edges [h] n n') n = SOME (n1,n2) ∧
+    ALOOKUP [h] n = SOME (n1',n2') ⇒
+    (n1' = n1)
+Proof
+  rpt strip_tac >>
+  PairCases_on ‘h’ >>
+  rpt strip_tac >>
+  gvs[merge_edges_def] >>
+  rgs[AllCaseEqs()] >>
+  gvs[]
+QED
+
+
+
+
+Theorem merge_edges_elim_same_l:        
+  ∀ edges l n n' n1 n2 n1' n2'.        
+    n1 ≠ n ∧
+    ALOOKUP (merge_edges edges n n') n = SOME (n1,n2) ∧
+    ALOOKUP edges n = SOME (n1',n2') ⇒
+    n1'=n1 
+Proof
+  Induct >-
+   gvs[] >>
+  rpt strip_tac >>
+  
+  rfs[Once merge_edges_list_cons] >>
+  
+  PairCases_on ‘h’ >>
+  rfs[Once ALOOKUP_APPEND] >>
+  
+  rgs[] >>
+  rgs[AllCaseEqs()] >>
+                    
+  rw[Once merge_edges_def] >>
+  rgs[Once merge_edges_def] >>
+  rgs[] >>
+  rgs[AllCaseEqs()] >>
+  
+  res_tac >>
+  metis_tac[merge_Theorem1]
+QED
+
+
+
+                
+
+Theorem eleminatble_correct_internal:
+  ∀ x vars_consumed vars r edges labels n n' n'' nl nr pred mv b rec.
+    consumed_dom_bdd vars_consumed (r,edges,labels) ∧
+    fv_in_BDD rec (r,edges,labels) (vars ⧺ vars_consumed) ∧
+    mv_dom_vars mv (vars ⧺ vars_consumed) ∧
+    BDD_ordered (r,edges,labels) vars_consumed ∧
+    BDD_WF (r,edges,labels) ∧
+    eleminatble (r,edges,labels) n n' ∧
+    n'' ≠ n' ∧
+    ALOOKUP edges n'' = SOME (nr,nl) ∧
+    ALOOKUP labels n'' = SOME (non_termn (SOME x,pred))
+    ⇒
+    (BDD_sem rec (r,edges,labels) mv n'' b ⇔
+       BDD_sem rec (r,ADELKEY n' (merge_edges edges n n'),ADELKEY n' labels) mv n'' b)
+Proof
+  
+  ntac 2 strip_tac >>
+  measureInduct_on `THE(INDEX_OF x vars_consumed)` >>
+  rpt strip_tac >>
+  
+  simp[Once BDD_sem_cases]>> gvs[] >>
+  
+  simp[Once EQ_SYM_EQ, Once BDD_sem_cases] >>
+  gvs[ALOOKUP_ADELKEY] >>
+  
+  gvs[from_formula_to_action_def] >>
+  Cases_on ‘ALOOKUP (merge_edges edges n n') n''’ >> gvs[] >|[
+    
+    
+    (*contr: in merged edges lookup is none , thus a leaf *)
+    assume_tac merge_lookup_none >>
+    first_x_assum (strip_assume_tac o (Q.SPECL [‘edges’,‘n’,‘n'’,‘n''’])) >>
+    gvs[]
+    ,
+        
+    (* in merged edges n'' is internal node  *)
+    PairCases_on ‘x'’ >> gvs[] >>      
+    Cases_on ‘ALOOKUP mv x’ >> gvs[] >> Cases_on ‘x'’ >> gvs[] >|[
+        
+        (*Case True*)
+        
+        Cases_on ‘nr=x'0’ >> gvs[]  >|[
+          
+          (*nr=x'0 means it did not change which makes it not the father of eliminated node, trivial case *)
+          
+          Cases_on ‘ALOOKUP edges nr’ >> gvs[] >|[
+            ‘n'≠nr’ by metis_tac[merge_edges_res] >>
+            metis_tac[mergable_correct_leaf]     
+            ,
+            
+            Cases_on ‘x'’ >> gvs[] >>
+            ‘MEM nr (dom_range_edges edges)’ by imp_res_tac lookup_edges_in_domain >>
+            ‘∃pred x'. ALOOKUP labels nr = SOME (non_termn (SOME x',pred))’ by
+              (imp_res_tac WF_imp_non_leaf_lbl >> gvs[]) >>
+            
+            gvs[] >>
+            subgoal ‘THE (INDEX_OF x' vars_consumed) < THE (INDEX_OF x vars_consumed)’ >-
+             (imp_res_tac ordered_for_two_labels) >>
+            
+            
+            first_x_assum (strip_assume_tac o (Q.SPECL [‘INDEX_OF (x':string) (vars_consumed: string list)’])) >>
+            rgs[PULL_FORALL] >>  
+            first_x_assum (strip_assume_tac o (Q.SPECL [‘x'’, ‘vars_consumed’, ‘vars’, ‘r’, ‘edges’, ‘labels’, ‘n’, ‘n'’,
+                                                        ‘nr’, ‘r'’, ‘q’,  ‘pred'’, ‘mv’, ‘b’])) >>
+            gvs[] >>
+            
+            ‘n'≠nr’ by metis_tac[merge_edges_res] >>
+            gvs[]
+          ]
+                                                 
+          ,
+          
+          
+          (*nr≠x'0, thus this is the parent of the node that disappeared, parent to n' *)
+          gvs[eleminatble_def] >>
+          
+          ‘x'0 = n ∧ nr = n' ’ by (imp_res_tac merge_parent_change >> metis_tac[]) >>
+          rgs[] >>
+          
+          
+          simp[Once EQ_SYM_EQ, Once BDD_sem_cases] >>
+          
+          ‘MEM n' (dom_range_edges edges)’ by imp_res_tac lookup_edges_in_domain >>
+          
+          subgoal ‘∃ x pred. ALOOKUP labels n' = SOME (non_termn (SOME x,pred))’ >-
+           ( metis_tac[WF_imp_non_leaf_lbl_abs,lookup_is_some_def] ) >>
+          gvs[] >>
+          
+          
+          subgoal ‘∃bool . ALOOKUP mv x' = SOME bool’ >-
+           (imp_res_tac consumed_dom_bdd_in_mv >> gvs[] ) >>
+          
+          Cases_on ‘bool’ >>  gvs[] >> ( (*includes both when x' = T and F *)
+            
+            Cases_on ‘ALOOKUP (merge_edges edges n n') n’ >|[
+                
+                ‘ALOOKUP edges n = NONE’ by (metis_tac [merge_lookup_none]) >>
+                metis_tac[mergable_correct_leaf]      
+                ,
+                
+                PairCases_on ‘x''’ >>
+                rename1 ‘ALOOKUP (merge_edges edges n n') n = SOME (n1,n2)’ >>
+                
+                ‘∃x''. ALOOKUP edges n = SOME x''’ by  (imp_res_tac merge_lookup_exists >> gvs[]) >>
+                PairCases_on ‘x''’ >> gvs[] >>
+                ‘x''0 ≠ n ∧ x''1 ≠ n’ by (imp_res_tac lookup_edges_not_parent >> gvs[]) >>
+                ‘n1 ≠ n' ∧ x'1 ≠ n' ∧ n2 ≠ n' ’ by (metis_tac[merge_edges_glue]) >>
+                Cases_on ‘n = n1’ >> gvs[] >|[
+                    
+                    (* by contr *)
+                    ‘x''0 = n'’ by imp_res_tac merge_parent_change >>
+                    rgs[] >>
+                    
+                    ‘∃ x pred. ALOOKUP labels n = SOME (non_termn (SOME x,pred))’ by metis_tac[WF_imp_non_leaf_lbl_abs,lookup_is_some_def]  >>
+                    
+                    subgoal ‘THE (INDEX_OF x' vars_consumed) < THE (INDEX_OF x'' vars_consumed)’ >-
+                     (imp_res_tac ordered_for_two_labels) >>
+                    subgoal ‘THE (INDEX_OF x'' vars_consumed) < THE (INDEX_OF x' vars_consumed)’ >-
+                     (imp_res_tac ordered_for_two_labels) >>
+                    gvs[]
+                    ,
+                    
+                    ‘x''0 = n1 ’ by metis_tac[merge_edges_elim_same_l] >>
+                    gvs[] >>
+                    
+                    simp[Once EQ_SYM_EQ, Once BDD_sem_cases] >>
+
+                    (* make subgoal *)
+                    subgoal ‘∃ x pred. ALOOKUP labels n = SOME (non_termn (SOME x,pred))’ >-
+                     ( metis_tac[WF_imp_non_leaf_lbl_abs,lookup_is_some_def]) >>
+                    
+                    subgoal ‘∃bool . ALOOKUP mv x'' = SOME bool’ >-
+                     ( imp_res_tac consumed_dom_bdd_in_mv >> gvs[] )  >>
+                    
+                    simp[Once EQ_SYM_EQ, Once BDD_sem_cases] >>
+                    ‘ALOOKUP (ADELKEY n' (merge_edges edges n n')) n = SOME (n1,n2)’ by metis_tac[delkey_alookup_imp_og] >>
+                    gvs[] >>
+                    
+                    ‘ALOOKUP (ADELKEY n' labels) n = SOME (non_termn (SOME x'',pred''))’ by metis_tac[delkey_alookup_imp_og] >>
+
+                    subgoal ‘THE (INDEX_OF x'' vars_consumed) < THE (INDEX_OF x vars_consumed)’ >-
+                     (
+                     ‘THE (INDEX_OF x' vars_consumed) < THE (INDEX_OF x vars_consumed)’ by (imp_res_tac ordered_for_two_labels) >>
+                     ‘THE (INDEX_OF x'' vars_consumed) < THE (INDEX_OF x' vars_consumed)’ by (imp_res_tac ordered_for_two_labels) >>
+                     gvs[]
+                     ) >>                    
+                    
+                    first_x_assum (strip_assume_tac o (Q.SPECL [‘INDEX_OF (x'':string) (vars_consumed: string list)’])) >>
+                    gvs[PULL_FORALL] >>
+                    first_x_assum (strip_assume_tac o (Q.SPECL [‘x''’, ‘vars_consumed’, ‘vars’, ‘r’, ‘edges’, ‘labels’, ‘n’, ‘n'’, ‘n’,
+                                                                ‘x''1’, ‘n1’, ‘pred''’, ‘mv’, ‘b’, ‘rec’])) >>
+                    gvs[] >>
+                    rgs[Once BDD_sem_cases] >>
+                    simp[Once EQ_SYM_EQ, Once BDD_sem_cases]
+                  ]
+              ]
+            )                           
+        ]
+        ,
+
+
+                
+        (*Case False *)
+        Cases_on ‘nl=x'1’ >> gvs[]  >|[
+          
+          (*nr=x'0 means it did not change which makes it not the father of eliminated node, trivial case *)
+          
+          Cases_on ‘ALOOKUP edges nl’ >> gvs[] >|[
+            ‘n'≠nl’ by metis_tac[merge_edges_res] >>
+            metis_tac[mergable_correct_leaf]     
+            ,
+            
+            Cases_on ‘x'’ >> gvs[] >>
+            ‘MEM nl (dom_range_edges edges)’ by imp_res_tac lookup_edges_in_domain >>
+            ‘∃pred x'. ALOOKUP labels nl = SOME (non_termn (SOME x',pred))’ by
+              (imp_res_tac WF_imp_non_leaf_lbl >> gvs[]) >>
+            
+            gvs[] >>
+            subgoal ‘THE (INDEX_OF x' vars_consumed) < THE (INDEX_OF x vars_consumed)’ >-
+             (imp_res_tac ordered_for_two_labels) >>
+            
+            
+            first_x_assum (strip_assume_tac o (Q.SPECL [‘INDEX_OF (x':string) (vars_consumed: string list)’])) >>
+            rgs[PULL_FORALL] >>  
+            first_x_assum (strip_assume_tac o (Q.SPECL [‘x'’, ‘vars_consumed’, ‘vars’, ‘r’, ‘edges’, ‘labels’, ‘n’, ‘n'’,
+                                                        ‘nl’, ‘r'’, ‘q’,  ‘pred'’, ‘mv’, ‘b’])) >>
+            gvs[] >>
+            
+            ‘n'≠nl’ by metis_tac[merge_edges_res] >>
+            gvs[]
+          ]
+                                                 
+          ,
+          
+          
+          (*nl≠x'1, thus this is the parent of the node that disappeared, parent to n' *)
+          gvs[eleminatble_def] >>
+          
+          ‘x'1 = n ∧ nl = n' ’ by (imp_res_tac merge_parent_change >> metis_tac[]) >>
+          rgs[] >>
+          
+          
+          simp[Once EQ_SYM_EQ, Once BDD_sem_cases] >>
+          
+          ‘MEM n' (dom_range_edges edges)’ by imp_res_tac lookup_edges_in_domain >>
+          
+          subgoal ‘∃ x pred. ALOOKUP labels n' = SOME (non_termn (SOME x,pred))’ >-
+           ( metis_tac[WF_imp_non_leaf_lbl_abs,lookup_is_some_def] ) >>
+          gvs[] >>
+          
+          
+          subgoal ‘∃bool . ALOOKUP mv x' = SOME bool’ >-
+           (imp_res_tac consumed_dom_bdd_in_mv >> gvs[] ) >>
+          
+          Cases_on ‘bool’ >>  gvs[] >> ( (*includes both when x' = T and F *)
+            
+            Cases_on ‘ALOOKUP (merge_edges edges n n') n’ >|[
+                
+                ‘ALOOKUP edges n = NONE’ by (metis_tac [merge_lookup_none]) >>
+                metis_tac[mergable_correct_leaf]      
+                ,
+                
+                PairCases_on ‘x''’ >>
+                rename1 ‘ALOOKUP (merge_edges edges n n') n = SOME (n1,n2)’ >>
+                
+                ‘∃x''. ALOOKUP edges n = SOME x''’ by  (imp_res_tac merge_lookup_exists >> gvs[]) >>
+                PairCases_on ‘x''’ >> gvs[] >>
+                ‘x''0 ≠ n ∧ x''1 ≠ n’ by (imp_res_tac lookup_edges_not_parent >> gvs[]) >>
+                Cases_on ‘n = n1’ >> gvs[] >|[
+                    
+                    (* by contr *)
+                    ‘x''0 = n'’ by imp_res_tac merge_parent_change >>
+                    rgs[] >>
+                    
+                    ‘∃ x pred. ALOOKUP labels n = SOME (non_termn (SOME x,pred))’ by metis_tac[WF_imp_non_leaf_lbl_abs,lookup_is_some_def]  >>
+                    
+                    subgoal ‘THE (INDEX_OF x' vars_consumed) < THE (INDEX_OF x'' vars_consumed)’ >-
+                     (imp_res_tac ordered_for_two_labels) >>
+                    subgoal ‘THE (INDEX_OF x'' vars_consumed) < THE (INDEX_OF x' vars_consumed)’ >-
+                     (imp_res_tac ordered_for_two_labels) >>
+                    gvs[]
+                    ,
+                    
+                    ‘x''0 = n1 ’ by metis_tac[merge_edges_elim_same_l] >>
+                    gvs[] >>
+                    
+                    simp[Once EQ_SYM_EQ, Once BDD_sem_cases] >>
+
+                    (* make subgoal *)
+                    subgoal ‘∃ x pred. ALOOKUP labels n = SOME (non_termn (SOME x,pred))’ >-
+                     ( metis_tac[WF_imp_non_leaf_lbl_abs,lookup_is_some_def]) >>
+                    
+                    subgoal ‘∃bool . ALOOKUP mv x'' = SOME bool’ >-
+                     ( imp_res_tac consumed_dom_bdd_in_mv >> gvs[] )  >>
+                    
+                    simp[Once EQ_SYM_EQ, Once BDD_sem_cases] >>
+                    ‘ALOOKUP (ADELKEY n' (merge_edges edges n n')) n = SOME (n1,n2)’ by metis_tac[delkey_alookup_imp_og] >>
+                    gvs[] >>
+                    
+                    ‘ALOOKUP (ADELKEY n' labels) n = SOME (non_termn (SOME x'',pred''))’ by metis_tac[delkey_alookup_imp_og] >>
+
+                    subgoal ‘THE (INDEX_OF x'' vars_consumed) < THE (INDEX_OF x vars_consumed)’ >-
+                     (
+                     ‘THE (INDEX_OF x' vars_consumed) < THE (INDEX_OF x vars_consumed)’ by (imp_res_tac ordered_for_two_labels) >>
+                     ‘THE (INDEX_OF x'' vars_consumed) < THE (INDEX_OF x' vars_consumed)’ by (imp_res_tac ordered_for_two_labels) >>
+                     gvs[]
+                     ) >>                    
+                    
+                    first_x_assum (strip_assume_tac o (Q.SPECL [‘INDEX_OF (x'':string) (vars_consumed: string list)’])) >>
+                    gvs[PULL_FORALL] >>
+                    first_x_assum (strip_assume_tac o (Q.SPECL [‘x''’, ‘vars_consumed’, ‘vars’, ‘r’, ‘edges’, ‘labels’, ‘n’, ‘n'’, ‘n’,
+                                                                ‘x''1’, ‘n1’, ‘pred''’, ‘mv’, ‘b’, ‘rec’])) >>
+                    gvs[] >>
+                    rgs[Once BDD_sem_cases] >>
+                    simp[Once EQ_SYM_EQ, Once BDD_sem_cases]
+                  ]
+              ]
+            )                          
+        ]
+      ]
+  ]
+
+QED
+        
 
 
  
 
+Theorem eleminatble_correct_eq:
+∀labels vars vars_consumed n'' r edges n' n mv b rec.
+consumed_dom_bdd vars_consumed (r,edges,labels) ∧
+fv_in_BDD rec (r,edges,labels) (vars++vars_consumed) ∧
+mv_dom_vars mv (vars ⧺ vars_consumed) ∧
+BDD_ordered (r,edges,labels) vars_consumed ∧
+BDD_WF (r,edges,labels) ∧
+eleminatble (r,edges,labels) n n' ∧ n'' ≠ n' ⇒
+(BDD_sem rec (r,edges,labels) mv n'' b ⇔
+        BDD_sem rec (r,ADELKEY n' (merge_edges edges n n'),ADELKEY n' labels)  mv n'' b)
+Proof
 
+  rpt strip_tac >>
+      
+  Cases_on ‘ALOOKUP edges n''’ >> gvs[] >|[
+    assume_tac  mergable_correct_leaf >> 
+    last_x_assum (strip_assume_tac o (Q.SPECL [‘labels’,‘n''’,‘r’, ‘edges’, ‘n'’, ‘n’, ‘mv’, ‘b’])) >>
+    gvs[]
+    ,
+    PairCases_on ‘x’ >>
+
+    subgoal ‘∃pred x'. ALOOKUP labels n'' = SOME (non_termn (SOME x',pred))’ >-
+     (
+     ‘MEM n'' (dom_range_edges edges)’ by imp_res_tac lookup_edges_in_domain >>
+     imp_res_tac WF_imp_non_leaf_lbl >> gvs[]
+     ) >>
+
+     
+   metis_tac[eleminatble_correct_internal]
+  ]
+QED
+
+          
+                           
+                
+ (* merge = eliminate defs*)       
+Theorem eliminate_correct:        
+  ∀ r edges labels vars vars_consumed n n' rec .
+    correct_sem rec (r,edges,labels) (vars++vars_consumed) ∧
+    BDD_WF (r,edges,labels) ∧
+    consumed_dom_bdd vars_consumed (r,edges,labels) ∧
+    BDD_ordered (r,edges,labels) vars_consumed ∧
+    fv_in_BDD rec (r,edges,labels) (vars++vars_consumed)  ∧
+    eleminatble (r,edges,labels) n n'
+    ==>
+    correct_sem rec (merge (r,edges,labels) n n')  (vars++vars_consumed)
+Proof
+  rpt strip_tac >>   
+  simp[Once correct_sem_def] >>
+  rpt strip_tac >>
+  
+  Cases_on ‘n' = n''’ >> gvs[] >|[
+    
+    gvs[merge_def] >>
+    ‘get_prop (ADELKEY n' labels) n' = NONE’ by gvs[get_prop_delkey_none] >> 
+    gvs[op_sem_def, get_prop_def] >>
+    gvs[AllCaseEqs()]>>
+
+    gvs[Once BDD_sem_cases]
+    ,
+
+
+    gvs[merge_def] >>
+    assume_tac eleminatble_correct_eq >>
+    first_x_assum (strip_assume_tac o (Q.SPECL [‘labels’, ‘vars’, ‘vars_consumed’, ‘n''’, ‘r’, ‘edges’, ‘n'’, ‘n’, ‘mv’, ‘b’, ‘rec’])) >>
+    gvs[] >>
+    
+    gvs[correct_sem_def] >>
+    res_tac >>
+    
+    metis_tac[op_sem_adel_key]
+  ]
+QED
+
+
+
+
+(*
+
+EVAL “mergable (0,[(0,1,2)],
+        [(0,non_termn (SOME "a",Or (Var "a") (Not (Var "a"))));
+         (1,termn (T,True)); (2,termn (T,True))]) 1 2”
+
+
+EVAL “merge (0,[(0,1,2)],
+        [(0,non_termn (SOME "a",Or (Var "a") (Not (Var "a"))));
+         (1,termn (T,True)); (2,termn (T,True))]) 1 2” 
+
+
+
+EVAL “eleminatble (0,[(0,1,1)],
+      [(0,non_termn (SOME "a",Or (Var "a") (Not (Var "a"))));
+       (1,termn (T,True))]) 1 0” 
         
+EVAL “merge (0,[(0,1,1)],
+      [(0,non_termn (SOME "a",Or (Var "a") (Not (Var "a"))));
+       (1,termn (T,True))]) 1 0” 
+
+*)
+
+(*
+EVAL “is_unique_var [(1,non_termn (SOME "x",p));(2,non_termn (SOME "x",p))] (1:num)” 
+*)
+
+
+       
 
 val _ = export_theory ();
